Nat.lean
@@ -6,25 +6,123 @@ private structure Sig where
   «Nat.zero» : Nat
   «Nat.succ» : Nat → Nat
   «Nat.rec₀» {motive : Nat → Prop} : motive «Nat.zero» → (∀ n, motive n → motive («Nat.succ» n)) → ∀ n, motive n
+  «Nat.rec₀_zero» {motive} zero succ : @«Nat.rec₀» motive zero succ «Nat.zero» = zero
+  «Nat.rec₀_succ» {motive} zero succ n : @«Nat.rec₀» motive zero succ («Nat.succ» n) = succ n (@«Nat.rec₀» motive zero succ n)
+  «Nat.rec₁» {motive : Nat → Type} : motive «Nat.zero» → (∀ n, motive n → motive («Nat.succ» n)) → ∀ n, motive n
+  «Nat.rec₁_zero» {motive} zero succ : @«Nat.rec₁» motive zero succ «Nat.zero» = zero
+  «Nat.rec₁_succ» {motive} zero succ n : @«Nat.rec₁» motive zero succ («Nat.succ» n) = succ n (@«Nat.rec₁» motive zero succ n)
+  «Nat.rec₂» {motive : Nat → Type 1} : motive «Nat.zero» → (∀ n, motive n → motive («Nat.succ» n)) → ∀ n, motive n
+  «Nat.rec₂_zero» {motive} zero succ : @«Nat.rec₂» motive zero succ «Nat.zero» = zero
+  «Nat.rec₂_succ» {motive} zero succ n : @«Nat.rec₂» motive zero succ («Nat.succ» n) = succ n (@«Nat.rec₂» motive zero succ n)
+  «Nat.zero_ne_succ» n : «Nat.zero» ≠ «Nat.succ» n
+  «Nat.succ_inj» {n m} : «Nat.succ» n = «Nat.succ» m → n = m
+  «Nat.ne_succ_self» {n} : n ≠ «Nat.succ» n
 
 private structure Sig' (Imp : Sig) where
   «Nat.rec» {motive : Imp.Nat → Sort u} : motive Imp.«Nat.zero» → (∀ n, motive n → motive (Imp.«Nat.succ» n)) → ∀ n, motive n
   «Nat.rec_zero» {motive} zero succ : @«Nat.rec» motive zero succ Imp.«Nat.zero» = zero
   «Nat.rec_succ» {motive} zero succ n : @«Nat.rec» motive zero succ (Imp.«Nat.succ» n) = succ n (@«Nat.rec» motive zero succ n)
 
-/-
-instance : Nonempty (Sig' Imp) := ⟨{
-  «Nat.rec» := λ {motive} zero succ n => Classical.choice <| @Sig.«Nat.rec₀» Imp (Nonempty <| motive ·) ⟨zero⟩ (⟨succ · <| Classical.choice ·⟩) n
-}⟩
--/
+attribute [elab_as_elim] Sig.«Nat.rec₀» Sig.«Nat.rec₁» Sig.«Nat.rec₂»
+attribute [simp] Sig.«Nat.rec₀_zero» Sig.«Nat.rec₀_succ» Sig.«Nat.rec₁_zero» Sig.«Nat.rec₁_succ» Sig.«Nat.rec₂_zero» Sig.«Nat.rec₂_succ»
 
-instance : Nonempty (Sig' Imp) :=
-  let rec' {motive : _ → _} (zero : motive _) (succ : ∀ n, motive n → motive _) := 
-    @Sig.«Nat.rec₀» Imp (λ n => ∃ x, (∀ (h : n = Imp.«Nat.zero»), h ▸ x = zero) ∧ (∀ n' (h : n = Imp.«Nat.succ» n'), h ▸ x = succ n' sorry)) ⟨zero, λ _ => rfl, sorry⟩ (λ n ih => ⟨succ n (Classical.choose ih), sorry, sorry⟩)
+instance : Nonempty (Sig'.{u} Imp) :=
+  let lt (n : Imp.«Nat») : Imp.«Nat» → Type := Imp.«Nat.rec₂» Empty λ m ih => n = m ⊕' ih
+  let le (n m : Imp.«Nat») : Type := n = m ⊕' lt n m
+  have not_lt_self {n} : lt n n → False := Imp.«Nat.rec₀» (by simp) (λ n ih h => by simp at h; cases h with | inl h => sorry | inr h => (conv at h => change lt (Imp.«Nat.succ» n) n); sorry) n
+  have subsingleton_lt {n m} (h₁ h₂ : lt n m) : h₁ = h₂ :=
+    @Sig.«Nat.rec₀» Imp
+      (λ m => (h₁ h₂ : lt n m) → h₁ = h₂)
+      (λ h₁ h₂ => by simp at h₁; cases h₁)
+      (λ m ih h₁ h₂ => by
+        rename_i M H₁ H₂; clear M H₁ H₂
+        dsimp at h₁ h₂ ih
+        have : _ = h₁ := cast_cast (by simp; rfl) (by simp) h₁; rw [← this]; clear this
+        generalize (cast _ h₁) = h₁'; clear h₁; rename _ => h₁
+        have : _ = h₂ := cast_cast (by simp; rfl) (by simp) h₂; rw [← this]; clear this
+        generalize (cast _ h₂) = h₂'; clear h₂; rename _ => h₂
+        congr
+        cases h₁ with
+        | inl h₁ =>
+          cases h₂ with
+          | inl h₂ => rfl
+          | inr h₂ => cases h₁; cases not_lt_self h₂
+        | inr h₁ =>
+          cases h₂ with
+          | inl h₂ => cases h₂; cases not_lt_self h₁
+          | inr h₂ => congr; apply ih
+      ) m h₁ h₂
+  have subsingleton_le {n m} (h₁ h₂ : le n m) : h₁ = h₂ := by
+    cases h₁ with
+    | inl h₁ =>
+      cases h₂ with
+      | inl h₂ => rfl
+      | inr h₂ => cases h₁; cases not_lt_self h₂
+    | inr h₁ =>
+      cases h₂ with
+      | inl h₂ => cases h₂; cases not_lt_self h₁
+      | inr h₂ => congr; apply subsingleton_lt
+  have lt_of_succ_le {n m} : le (Imp.«Nat.succ» n) m → lt n m := λ h => sorry
+  have lt_succ_of_le {n m} : le n m → lt n (Imp.«Nat.succ» m) := λ h => sorry
+  have not_lt_zero {n} : lt n Imp.«Nat.zero» → False := λ h => by simp [Sig.«Nat.rec₂_zero»] at h; cases h
+  have le_of_lt_succ {n m} : lt n (Imp.«Nat.succ» m) → le n m := λ h => sorry
+  have le_succ_of_lt {n m} : lt n m → le (Imp.«Nat.succ» n) m := λ h => sorry
+  have zero_le {n} : le Imp.«Nat.zero» n := sorry
+  have lt_succ_self {n} : lt n (Imp.«Nat.succ» n) := sorry
+  have rec' {motive : Imp.«Nat» → Sort u} (zero : motive Imp.«Nat.zero») (succ : ∀ n, motive n → motive (Imp.«Nat.succ» n)) :=
+    @Sig.«Nat.rec₀» Imp
+      (λ n => ∃ (f : ∀ m, le m n → motive m), f Imp.«Nat.zero» zero_le = zero ∧ ∀ m h, f (Imp.«Nat.succ» m) (le_succ_of_lt h) = succ m (f m (PSum.inr h)))
+      ⟨λ m h => h.casesOn (· ▸ zero) (nomatch not_lt_zero ·), by dsimp; apply Eq.trans; apply congrArg; apply subsingleton_le; exact PSum.inl rfl; rfl, λ _ h => not_lt_zero h |>.elim⟩
+      λ n ih => ⟨λ m h => h.casesOn (· ▸ succ n (Classical.choose ih n (PSum.inl rfl))) (Classical.choose ih m <| le_of_lt_succ ·),
+        by dsimp; apply Eq.trans; apply congrArg; apply subsingleton_le; apply PSum.inr; apply lt_succ_of_le; apply zero_le
+           dsimp; apply Eq.trans; apply congrArg; apply subsingleton_le; apply zero_le
+           exact Classical.choose_spec ih |>.left,
+        by intro m h
+           dsimp
+           cases le_of_lt_succ h with
+           | inl h =>
+             cases h
+             apply Eq.trans
+             . apply congrArg; apply subsingleton_le; apply PSum.inl; rfl
+             . apply congrArg (succ n <| Classical.choose ih n ·); apply subsingleton_le
+           | inr h =>
+             have h' : lt (Sig.«Nat.succ» Imp m) (Sig.«Nat.succ» Imp n) := lt_succ_of_le <| le_succ_of_lt h
+             apply Eq.trans; apply congrArg; apply subsingleton_le; exact PSum.inr h'
+             dsimp
+             have := Classical.choose_spec ih |>.right m h
+             apply Eq.trans (Eq.trans _ this) _
+             . apply congrArg; apply subsingleton_le
+             . apply congrArg (succ m <| Classical.choose ih m ·); apply subsingleton_le
+        ⟩
   ⟨{
-    «Nat.rec» := λ zero succ n => Classical.choose (rec' zero succ n)
-    «Nat.rec_zero» := λ zero succ => Classical.choose_spec (rec' zero succ Imp.«Nat.zero») |>.left rfl
-    «Nat.rec_succ» := λ zero succ n => by dsimp only []; show Classical.choose (rec' zero succ (Imp.«Nat.succ» n)) = succ n (Classical.choose (rec' zero succ n)); have := Classical.choose_spec (rec' zero succ (Imp.«Nat.succ» n)) |>.right n rfl; dsimp only [] at this; apply this.trans; clear this; sorry
+    «Nat.rec» := λ zero succ n => Classical.choose (rec' zero succ n) n (PSum.inl rfl)
+    «Nat.rec_zero» := λ zero succ => by
+      apply Eq.trans _ <| Classical.choose_spec (rec' zero succ Imp.«Nat.zero») |>.left
+      apply congrArg
+      apply subsingleton_le
+    «Nat.rec_succ» := λ zero succ n => by
+      have := Classical.choose_spec (rec' zero succ (Imp.«Nat.succ» n)) |>.right n lt_succ_self
+      simp
+      apply Eq.trans (Eq.trans _ this) _
+      . apply congrArg; apply subsingleton_le
+      . apply congrArg
+        clear this
+        induction n using Sig.«Nat.rec₀»
+        next =>
+          have := Classical.choose_spec (rec' zero succ (Imp.«Nat.succ» Imp.«Nat.zero»)) |>.left
+          apply Eq.trans (Eq.trans _ this) _
+          . apply congrArg; apply subsingleton_le
+          . have := Classical.choose_spec (rec' zero succ Imp.«Nat.zero») |>.left
+            apply Eq.symm
+            apply Eq.trans _ this
+            apply congrArg; apply subsingleton_le
+        next n ih =>
+          have := Classical.choose_spec (rec' zero succ (Imp.«Nat.succ» (Imp.«Nat.succ» n))) |>.right n sorry
+          apply Eq.trans (Eq.trans _ this) _
+          . apply congrArg; apply subsingleton_le
+          . clear this
+            have := Classical.choose_spec (rec' zero succ (Imp.«Nat.succ» (Imp.«Nat.succ» n))) |>.right n sorry
+            sorry
   }⟩
 
 private def Impl : Sig where
@@ -32,32 +130,28 @@ private def Impl : Sig where
   «Nat.zero» := .zero
   «Nat.succ» := .succ
   «Nat.rec₀» := @Nat.rec
+  «Nat.rec₀_zero» _ _ := rfl
+  «Nat.rec₀_succ» _ _ _ := rfl
+  «Nat.rec₁» := @Nat.rec
+  «Nat.rec₁_zero» _ _ := rfl
+  «Nat.rec₁_succ» _ _ _ := rfl
+  «Nat.rec₂» := @Nat.rec
+  «Nat.rec₂_zero» _ _ := rfl
+  «Nat.rec₂_succ» _ _ _ := rfl
+  «Nat.zero_ne_succ» _ := (nomatch ·)
+  «Nat.succ_inj» := Nat.succ.inj
+  «Nat.ne_succ_self» := (nomatch ·)
 
 private def Impl' : Sig' Impl where
   «Nat.rec» := @Nat.rec
   «Nat.rec_zero» _ _ := rfl
   «Nat.rec_succ» _ _ _ := rfl
 
-private opaque Imp₁ : Sig := Impl
-private opaque Imp₁' : Sig' Imp₁ := unsafe opaque_def% Imp₁ ▸ Impl'
-def Nat₁ : Type := Imp₁.Nat
-def Nat₁.zero : Nat₁ := Imp₁.«Nat.zero»
-def Nat₁.succ : Nat₁ → Nat₁ := Imp₁.«Nat.succ»
-def Nat₁.rec {motive : Nat₁ → Sort u} : motive .zero → (∀ n, motive n → motive n.succ) → ∀ n, motive n := Imp₁'.«Nat.rec»
-@[simp] theorem Nat₁.rec_zero : ∀ zero succ, @Nat₁.rec motive zero succ .zero = zero := Imp₁'.«Nat.rec_zero»
-@[simp] theorem Nat₁.rec_succ : ∀ zero succ n, @Nat₁.rec motive zero succ (.succ n) = succ n (@Nat₁.rec motive zero succ n) := Imp₁'.«Nat.rec_succ»
-
-private opaque Imp₂ : Sig := Impl
-private opaque Imp₂' : Sig' Imp₂ := unsafe opaque_def% Imp₂ ▸ Impl'
-def Nat₂ : Type := Imp₂.Nat
-def Nat₂.zero : Nat₂ := Imp₂.«Nat.zero»
-def Nat₂.succ : Nat₂ → Nat₂ := Imp₂.«Nat.succ»
-def Nat₂.rec {motive : Nat₂ → Sort u} : motive .zero → (∀ n, motive n → motive n.succ) → ∀ n, motive n := Imp₂'.«Nat.rec»
-@[simp] theorem Nat₂.rec_zero : ∀ zero succ, @Nat₂.rec motive zero succ .zero = zero := Imp₂'.«Nat.rec_zero»
-@[simp] theorem Nat₂.rec_succ : ∀ zero succ n, @Nat₂.rec motive zero succ (.succ n) = succ n (@Nat₂.rec motive zero succ n) := Imp₂'.«Nat.rec_succ»
-
-example : Nat₁ ≃ Nat₂ where
-  toFun := Nat₁.rec .zero λ _ => .succ
-  invFun := Nat₂.rec .zero λ _ => .succ
-  left_inv := Nat₁.rec (by simp) λ _ hn => by simp [hn]
-  right_inv := Nat₂.rec (by simp) λ _ hn => by simp [hn]
+private opaque Imp : Sig := Impl
+private opaque Imp' : Sig' Imp := unsafe opaque_def% Imp ▸ Impl'
+def Nat' : Type := Imp.Nat
+def Nat'.zero : Nat' := Imp.«Nat.zero»
+def Nat'.succ : Nat' → Nat' := Imp.«Nat.succ»
+@[elab_as_elim] def Nat'.rec {motive : Nat' → Sort u} : (zero : motive .zero) → (succ : ∀ n, motive n → motive n.succ) → ∀ n, motive n := Imp'.«Nat.rec»
+@[simp] theorem Nat'.rec_zero : ∀ zero succ, @Nat'.rec motive zero succ .zero = zero := Imp'.«Nat.rec_zero»
+@[simp] theorem Nat'.rec_succ : ∀ zero succ n, @Nat'.rec motive zero succ (.succ n) = succ n (@Nat'.rec motive zero succ n) := Imp'.«Nat.rec_succ»
