IndSig.lean
@@ -1,0 +1,30 @@
+import Mathlib.Logic.Equiv.Defs
+
+class Inductive (α : Type u) (F : Type u → Type v) [Functor F] where
+  fold (x : F α) : α
+  recursor {τ} (f : F τ → τ) (a : α) : τ
+  rec_fold f x : @recursor τ f (fold x) = f (recursor f <$> x)
+
+instance : Inductive Nat Option where
+  fold
+    | none => .zero
+    | some n => .succ n
+  recursor f := Nat.rec (f none) λ _ t => f <| some t
+  rec_fold _
+    | none => rfl
+    | some _ => rfl
+
+instance : Functor (Option <| α × ·) where
+  map f
+    | none => none
+    | some (a, x) => some (a, f x)
+
+noncomputable
+instance : Inductive (List α) (Option <| α × ·) where
+  fold
+    | none => .nil
+    | some (a, l) => .cons a l
+  recursor f := List.rec (f none) λ a _ t => f <| some (a, t)
+  rec_fold _
+    | none => rfl
+    | some _ => rfl
