Nat3.lean
@@ -1,0 +1,87 @@
+import Common.Meta
+import Mathlib.Logic.Equiv.Defs
+
+structure Sig where
+  Nat : Type
+  «Nat.zero» : Nat
+  «Nat.succ» : Nat → Nat
+  «Nat.rec₀» {motive : Nat → Prop} : motive «Nat.zero» → (∀ n, motive n → motive («Nat.succ» n)) → ∀ n, motive n
+
+structure Sig' (Imp : Sig) where
+  «Nat.rec» {motive : Imp.Nat → Sort u} : motive Imp.«Nat.zero» → (∀ n, motive n → motive (Imp.«Nat.succ» n)) → ∀ n, motive n
+  «Nat.rec_zero» {motive} zero succ : @«Nat.rec» motive zero succ Imp.«Nat.zero» = zero
+  «Nat.rec_succ» {motive} zero succ n : @«Nat.rec» motive zero succ (Imp.«Nat.succ» n) = succ n (@«Nat.rec» motive zero succ n)
+
+attribute [elab_as_elim] Sig.«Nat.rec₀» Sig'.«Nat.rec»
+attribute [simp] Sig'.«Nat.rec_zero» Sig'.«Nat.rec_succ»
+
+instance : Nonempty (Sig'.{u} Imp) :=
+  have rec₀ {motive : Imp.Nat → Sort (max 1 u)} (zero : motive Imp.«Nat.zero») (succ : ∀ n, motive n → motive (Imp.«Nat.succ» n)) n : motive n :=
+    Classical.choice <| Imp.«Nat.rec₀» ⟨zero⟩ (⟨succ · <| Classical.choice ·⟩) n
+  have rec {motive : Imp.Nat → Sort u} (zero : motive Imp.«Nat.zero») (succ : ∀ n, motive n → motive (Imp.«Nat.succ» n)) :=
+    @Sig.«Nat.rec₀» Imp
+      (λ n => ∃ x : motive n, @rec₀ (λ m => motive m → Prop) (λ x => x = zero) (λ n ih x => ∃ y, x = succ n y ∧ ih y) n x)
+      ⟨zero, by dsimp; sorry⟩
+      λ n hn => ⟨succ n (Classical.choose hn), sorry⟩
+  ⟨{
+    «Nat.rec» := λ zero succ n => Classical.choose <| rec zero succ n
+    «Nat.rec_zero» := λ zero succ => have := Classical.choose_spec <| rec zero succ Imp.«Nat.zero»; by dsimp only []; sorry
+    «Nat.rec_succ» := λ zero succ n => have := Classical.choose_spec <| rec zero succ (Imp.«Nat.succ» n); by dsimp only []; sorry
+  }⟩
+
+def Impl : Sig where
+  Nat := Nat
+  «Nat.zero» := .zero
+  «Nat.succ» := .succ
+  «Nat.rec₀» := @Nat.rec
+
+def Impl' : Sig' Impl where
+  «Nat.rec» := @Nat.rec
+  «Nat.rec_zero» _ _ := rfl
+  «Nat.rec_succ» _ _ _ := rfl
+
+opaque Imp₁ : Sig := Impl
+opaque Imp₁' : Sig' Imp₁ := unsafe opaque_def% Imp₁ ▸ Impl'
+
+opaque Imp₂ : Sig := Impl
+opaque Imp₂' : Sig' Imp₂ := unsafe opaque_def% Imp₂ ▸ Impl'
+
+structure Sig.Equiv (Imp₁ Imp₂ : Sig) where
+  equiv : Imp₁.Nat ≃ Imp₂.Nat
+  toFun_zero : equiv.toFun Imp₁.«Nat.zero» = Imp₂.«Nat.zero»
+  invFun_zero : equiv.invFun Imp₂.«Nat.zero» = Imp₁.«Nat.zero»
+  toFun_succ n : equiv.toFun (Imp₁.«Nat.succ» n) = Imp₂.«Nat.succ» (equiv.toFun n)
+  invFun_succ n : equiv.invFun (Imp₂.«Nat.succ» n) = Imp₁.«Nat.succ» (equiv.invFun n)
+
+structure Sig'.Equiv (Imp₁' : Sig' Imp₁) (Imp₂' : Sig' Imp₂) where
+  equiv : Sig.Equiv Imp₁ Imp₂
+  toFun_rec {motive} zero succ n : @Sig'.«Nat.rec» Imp₁ Imp₁' (motive <| equiv.equiv.toFun ·) (equiv.toFun_zero ▸ zero : motive _) (λ n ih => (equiv.toFun_succ n ▸ succ (equiv.equiv.toFun n) ih : motive _)) n = @Sig'.«Nat.rec» Imp₂ Imp₂' motive zero succ (equiv.equiv.toFun n)
+  invFun_rec {motive} zero succ n : @Sig'.«Nat.rec» Imp₂ Imp₂' (motive <| equiv.equiv.invFun ·) (equiv.invFun_zero ▸ zero : motive _) (λ n ih => (equiv.invFun_succ n ▸ succ (equiv.equiv.invFun n) ih : motive _)) n = @Sig'.«Nat.rec» Imp₁ Imp₁' motive zero succ (equiv.equiv.invFun n)
+
+theorem swap_eq_rec {β : α → _} {a a'} (h : a = a') {b : β a} {b' : β a'} : h ▸ b' = b → h ▸ b = b' :=
+  by cases h; exact .symm
+
+theorem rec_cast {n n' : Imp.Nat} (h : n = n') : h ▸ @Sig'.«Nat.rec» Imp Imp' motive zero succ n = @Sig'.«Nat.rec» Imp Imp' motive zero succ n' :=
+  by cases h; rfl
+
+theorem Imp₁'_Equiv_Imp₂' : Imp₁'.Equiv Imp₂' where
+  equiv.equiv.toFun := Imp₁'.«Nat.rec» Imp₂.«Nat.zero» λ _ => Imp₂.«Nat.succ»
+  equiv.equiv.invFun := Imp₂'.«Nat.rec» Imp₁.«Nat.zero» λ _ => Imp₁.«Nat.succ»
+  equiv.equiv.left_inv := Imp₁'.«Nat.rec» (by simp) λ _ => by simp; apply congrArg
+  equiv.equiv.right_inv := Imp₂'.«Nat.rec» (by simp) λ _ => by simp; apply congrArg
+  equiv.toFun_zero := by simp
+  equiv.invFun_zero := by simp
+  equiv.toFun_succ := by simp
+  equiv.invFun_succ := by simp
+  toFun_rec {motive} zero succ n := by
+    dsimp only []
+    refine Imp₁'.«Nat.rec» ?_ (λ _ _ => ?_) n <;> clear n
+      <;> simp <;> apply swap_eq_rec
+      <;> (apply Eq.trans; apply rec_cast; simp)
+    apply Eq.symm; congr
+  invFun_rec {motive} zero succ n := by
+    dsimp only []
+    refine Imp₂'.«Nat.rec» ?_ (λ _ _ => ?_) n <;> clear n
+      <;> simp <;> apply swap_eq_rec
+      <;> (apply Eq.trans; apply rec_cast; simp)
+    apply Eq.symm; congr
